theories/traversable_stack.v
@@ -1,0 +1,298 @@
+From iris.proofmode Require Import tactics.
+From iris.algebra Require Import auth excl.
+From iris.base_logic.lib Require Import invariants.
+From intensional.heap_lang Require Import lifting proofmode notation.
+From intensional.heap_lang Require Import adequacy.
+Set Default Proof Using "Type".
+
+Definition create_spec `{!heapG Σ} P0 (Stack: list val → val → iProp Σ) (create: val) : iProp Σ :=
+  {{{ P0 }}}
+    create #()
+  {{{ s, RET s; Stack [] s }}}.
+
+Definition push_spec `{!heapG Σ} (Stack: list val → val → iProp Σ) (push: val) : iProp Σ :=
+  ∀ l s x,
+     {{{ Stack l s }}}
+       push s x
+     {{{ RET #(); Stack (x :: l) s }}}.
+
+Definition pop_spec `{!heapG Σ} (Stack: list val → val → iProp Σ) (pop: val) : iProp Σ :=
+  ∀ l s,
+   {{{ Stack l s }}}
+     pop s
+   {{{ v, RET v;
+     match l with
+     | [] => ⌜ v = #() ⌝ ∗ Stack [] s
+     | x :: l' => ⌜ v = x ⌝ ∗ Stack l' s
+     end }}}.
+
+Definition foreach_spec `{!heapG Σ} (Stack: list val → val → iProp Σ) (foreach: val) : iProp Σ :=
+  ∀ l s (f: val) (I: list val → iProp Σ),
+  {{{ (∀ p x,
+        ⌜(p ++ [x]) `prefix_of` l⌝ →
+        {{{ I p }}} f x {{{ RET #(); I (p ++ [x]) }}}) ∗
+      Stack l s ∗ I []
+  }}}
+    foreach s f
+  {{{ RET #(); Stack l s ∗ I l }}}.
+
+Definition stacklib_spec `{!heapG Σ} (P0 : iProp Σ) (lib: val): iProp Σ :=
+  ∃ (Stack : list val → val → iProp Σ),
+    match lib with
+    | (create, push, pop, foreach)%V =>
+      create_spec P0 Stack create ∗
+      push_spec Stack push ∗
+      pop_spec Stack pop ∗
+      foreach_spec Stack foreach
+    | _ => False
+    end.
+
+Instance stacklib_persistent `{!heapG Σ} P0 lib : Persistent (stacklib_spec P0 lib).
+Proof.
+  apply bi.exist_persistent. intro.
+  repeat case_match; typeclasses eauto.
+Qed.
+
+
+Section Trace.
+
+Definition traversal_trace (f: val) (l: list val): list event :=
+  l ≫= (λ x, [("call:foreach_client", (f, x)%V); ("ret:foreach_client", f)]).
+
+Inductive good_trace_for : list val → list event → Prop :=
+| good_trace_for_nil: good_trace_for [] []
+| good_trace_for_push x l t:
+    good_trace_for l t →
+    good_trace_for (x :: l) (t ++ [("call:push", x); ("ret:push", #())])
+| good_trace_for_pop_nil t:
+    good_trace_for [] t →
+    good_trace_for [] (t ++ [("call:pop", #()); ("ret:pop", #())])
+| good_trace_for_pop x l t:
+    good_trace_for (x :: l) t →
+    good_trace_for l (t ++ [("call:pop", #()); ("ret:pop", x)])
+| good_trace_for_foreach l t f:
+    good_trace_for l t →
+    good_trace_for l (t ++ [("call:foreach", f)]
+                        ++ traversal_trace f l
+                        ++ [("ret:foreach", #())])
+.
+
+Definition good_trace (t: list event) :=
+  ∃ l t', t `prefix_of` t' ∧ good_trace_for l t'.
+
+Lemma good_trace_nil : good_trace [].
+Proof. eexists [],[]. split; eauto. constructor. Qed.
+
+Lemma traversal_trace_app f l l' :
+  traversal_trace f (l ++ l') = traversal_trace f l ++ traversal_trace f l'.
+Proof. unfold traversal_trace. apply bind_app. Qed.
+
+Lemma traversal_trace_prefix f l l' :
+  l `prefix_of` l' →
+  traversal_trace f l `prefix_of` traversal_trace f l'.
+Proof.
+  revert l'. induction l as [| x l]; cbn; intros l'.
+  { intros [? ->]. cbn. eexists; eauto. }
+  { intros [? ->]. cbn. do 2 apply prefix_cons.
+    rewrite bind_app. by apply prefix_app_r. }
+Qed.
+
+End Trace.
+
+
+Module Wrap.
+Section S.
+Context {Σ: gFunctors}.
+Context `{heapG Σ}.
+Context (N: namespace).
+
+Context (stack_impl: list val → val → iProp Σ).
+Context (push_impl pop_impl create_impl foreach_impl: val).
+
+Definition push : val :=
+  λ: "s" "x",
+    Emit "call:push" "x" ;;
+    push_impl "s" "x" ;;
+    Emit "ret:push" #().
+
+Definition pop : val :=
+  λ: "s",
+    Emit "call:pop" #() ;;
+    let: "r" := pop_impl "s" in
+    Emit "ret:pop" "r" ;;
+    "r".
+
+Definition create : val :=
+  create_impl.
+
+Definition foreach : val :=
+  λ: "s" "f",
+    Emit "call:foreach" "f" ;;
+    foreach_impl "s" (λ: "x",
+      Emit "call:foreach_client" ("f", "x") ;;
+      "f" "x" ;;
+      Emit "ret:foreach_client" "f"
+    ) ;;
+    Emit "ret:foreach" #().
+
+Definition stack_val (l: list val) (s: val): iProp Σ :=
+  stack_impl l s ∗ trace_inv N good_trace ∗
+  ∃ t, ⌜good_trace_for l t⌝ ∗ trace_is t.
+
+Lemma create_correct P0 :
+  create_spec P0 stack_impl create_impl -∗
+  create_spec (P0 ∗ trace_is [] ∗ trace_inv N good_trace) stack_val create.
+Proof.
+  iIntros "#create_impl_spec". iModIntro.
+  iIntros (φ) "(H0 & Htr & HI) Hφ". unfold create.
+  iApply ("create_impl_spec" with "[$]").
+  iIntros "!>" (?) "?". iApply "Hφ". rewrite /stack_val.
+  iFrame. iExists []. iFrame. iPureIntro. apply good_trace_for_nil.
+Qed.
+
+Lemma push_correct :
+  push_spec stack_impl push_impl -∗
+  push_spec stack_val push.
+Proof.
+  iIntros "#push_impl_spec" (l s x) "!>".
+  iIntros (φ) "Hs Hφ". unfold push.
+  iDestruct "Hs" as "(Hs & #HI & Htr)". iDestruct "Htr" as (t) "(Hgood & Ht)".
+  iDestruct "Hgood" as %Hgood.
+  wp_pures. wp_bind (Emit _ _).
+  iApply (wp_emit with "[$Ht $HI]"); eauto.
+  { do 2 eexists. split; cycle 1.
+    by eapply good_trace_for_push, Hgood.
+    apply prefix_app. eexists; eauto. }
+  iIntros "!> Ht". wp_pures. wp_bind (push_impl _ _).
+  iApply ("push_impl_spec" with "Hs"). iIntros "!> Hs".
+  wp_pures.
+  iApply (wp_emit with "[$Ht $HI]"); eauto.
+  { do 2 eexists. split; [reflexivity|].
+    rewrite -app_assoc /=. by eapply good_trace_for_push. }
+  iIntros "!> Ht". iApply "Hφ".
+  rewrite /stack_val; iFrame "HI∗".
+  iExists _; iFrame. iPureIntro.
+  rewrite -app_assoc /=. by eapply good_trace_for_push.
+Qed.
+
+Lemma pop_correct :
+  pop_spec stack_impl pop_impl -∗
+  pop_spec stack_val pop.
+Proof.
+  iIntros "#pop_impl_spec" (l s) "!>".
+  iIntros (φ) "Hs Hφ". unfold pop.
+  iDestruct "Hs" as "(Hs & #HI & Htr)". iDestruct "Htr" as (t) "(Hgood & Ht)".
+  iDestruct "Hgood" as %Hgood.
+  wp_pures. wp_bind (Emit _ _).
+  iApply (wp_emit with "[$Ht $HI]"); eauto.
+  { destruct l; eexists _,_; split;
+    [| by eapply good_trace_for_pop_nil |
+     | by eapply good_trace_for_pop ];
+    eexists; rewrite -app_assoc //=. }
+  iIntros "!> Ht". wp_pures. wp_bind (pop_impl _).
+  iApply ("pop_impl_spec" with "Hs"). iIntros "!>" (v) "Hs".
+  wp_pures. wp_bind (Emit _ _).
+  destruct l as [|x l'].
+  { iDestruct "Hs" as "(-> & Hs)".
+    iApply (wp_emit with "[$Ht $HI]"); eauto.
+    { rewrite -app_assoc /=. eexists _,_. split.
+      2: eapply good_trace_for_pop_nil; eauto. eauto. }
+    iIntros "!> Ht". wp_pures. iApply "Hφ". iSplitR; first done.
+    rewrite /stack_val; iFrame "HI∗".
+    iExists _. iFrame. iPureIntro.
+    rewrite -app_assoc/=. by apply good_trace_for_pop_nil. }
+  { iDestruct "Hs" as "(-> & Hs)".
+    iApply (wp_emit with "[$Ht $HI]"); eauto.
+    { rewrite -app_assoc /=. eexists _,_. split.
+      2: eapply good_trace_for_pop; eauto. eauto. }
+    iIntros "!> Ht". wp_pures. iApply "Hφ". iSplitR; first done.
+    rewrite /stack_val; iFrame "HI∗".
+    iExists _. iFrame. iPureIntro.
+    rewrite -app_assoc/=. by apply good_trace_for_pop. }
+Qed.
+
+Lemma foreach_correct :
+  foreach_spec stack_impl foreach_impl -∗
+  foreach_spec stack_val foreach.
+Proof.
+  iIntros "#foreach_impl_spec" (l s f I) "!>".
+  iIntros (φ) "(#Hf & Hs & HfI) Hφ". unfold foreach.
+  iDestruct "Hs" as "(Hs & #HI & Htr)". iDestruct "Htr" as (t) "(Hgood & Ht)".
+  iDestruct "Hgood" as %Hgood.
+  wp_pures. wp_bind (Emit _ _).
+  iApply (wp_emit with "[$Ht HI]"); eauto.
+  { eexists _,_; split. 2: by eapply good_trace_for_foreach.
+    apply prefix_app. eexists; eauto. }
+  iIntros "!> Ht". wp_pures. wp_bind (foreach_impl _ _).
+  unfold foreach_spec.
+  pose (λ p, I p ∗ trace_is (t ++ [("call:foreach", f)] ++ traversal_trace f p))%I as I'.
+  iApply ("foreach_impl_spec" $! _ _ _ I' with "[$Hs $HfI $Ht]").
+  { iIntros (p x Hpl φ') "!> HfI Hφ'". wp_pures. wp_bind (Emit _ _).
+    rewrite {1}/I'. iDestruct "HfI" as "(HfI & Htr)".
+    iApply (wp_emit with "[$Htr $HI]"); eauto.
+    { rewrite -!app_assoc. eexists _,_. split.
+      2: by apply good_trace_for_foreach.
+      do 2 apply prefix_app. apply prefix_app_r. transitivity (traversal_trace f (p ++ [x])).
+      2: by apply traversal_trace_prefix.
+      rewrite traversal_trace_app /=. apply prefix_app. eexists; eauto. }
+    iIntros "!> Htr". wp_pures. wp_bind (f x).
+    iApply ("Hf" with "[] HfI"); eauto. iIntros "!> HfI". wp_pures.
+    iApply (wp_emit with "[$Htr $HI]"); eauto.
+    { rewrite -!app_assoc. eexists _,_. split.
+      2: by apply good_trace_for_foreach.
+      do 2 apply prefix_app. apply prefix_app_r. transitivity (traversal_trace f (p ++ [x])).
+      2: by apply traversal_trace_prefix.
+      rewrite traversal_trace_app /=. apply prefix_app. eexists; eauto. }
+    iIntros "!> Htr". iApply "Hφ'". rewrite /I' traversal_trace_app /= -!app_assoc. iFrame. }
+  iIntros "!> (Hs & (HI' & Htr))". wp_pures.
+  iApply (wp_emit with "[Htr HI]"); eauto.
+  { eexists _,_. split; eauto. rewrite -app_assoc. by eapply good_trace_for_foreach. }
+  iIntros "!> Htr". iApply "Hφ". iFrame "HI∗". iExists _. iFrame. iPureIntro.
+  rewrite -app_assoc. by apply good_trace_for_foreach.
+Qed.
+
+End S.
+
+Definition lib (lib_impl: val): val :=
+  match lib_impl with
+  | (create_impl, push_impl, pop_impl, foreach_impl)%V =>
+    (create create_impl, push push_impl, pop pop_impl, foreach foreach_impl)
+  | _ => #()
+  end.
+
+Lemma correct `{!heapG Σ} N P0 (lib_impl: val):
+  stacklib_spec P0 lib_impl -∗
+  stacklib_spec (P0 ∗ trace_is [] ∗ trace_inv N good_trace) (lib lib_impl).
+Proof.
+  iIntros "#S". iDestruct "S" as (stack_val_impl) "S".
+  repeat case_match; eauto. iDestruct "S" as "(Hcreate & Hpush & Hpop & Hforeach)".
+  subst. unfold stacklib_spec.
+  iExists (stack_val N stack_val_impl). repeat iSplit.
+  iApply create_correct; eauto.
+  iApply push_correct; eauto.
+  iApply pop_correct; eauto.
+  iApply foreach_correct; eauto.
+Qed.
+
+End Wrap.
+
+
+Definition stacklibN := nroot .@ "traversable_stacklib".
+Definition empty_state : state := Build_state ∅ [] ∅.
+
+Lemma wrap_stacklib_correct {Σ} `{heapPreG Σ} (e: val → expr) (lib: val):
+  (⊢ ∀ `{heapG Σ}, stacklib_spec True lib) →
+  (⊢ ∀ `{heapG Σ} P lib, stacklib_spec P lib -∗ {{{ P }}} e lib {{{ v, RET v; True }}}) →
+  ∀ σ' e',
+    rtc erased_step ([(#();; e (Wrap.lib lib))%E], empty_state) (e', σ') →
+    good_trace (trace σ').
+Proof.
+  intros Hlib Hctx σ' e' Hsteps.
+  eapply (@module_invariance Σ _ stacklibN (@stacklib_spec Σ) True e #() (Wrap.lib lib)
+                            good_trace empty_state).
+  { cbn. apply good_trace_nil. }
+  { iIntros (? ? ?) "?". by iApply Hctx. }
+  { iIntros (? _) "!>". iApply wp_value; eauto. }
+  { iIntros (?). iApply Wrap.correct. iApply Hlib. }
+  eauto.
+Qed.
